Towards renameApart for mutual.

RenameApart.v
@@ -9,6 +9,27 @@ Set Implicit Arguments.
     a variable fresh for G at every binder, records the choice in ϱ,
     and renames all variables according to ϱ *)
 
+Definition renameApartFStep (renameApart':env var -> set var -> stmt -> set var * stmt) G ϱ :=
+  (fun Ys'G (Zs:params*stmt) =>
+     let Y := fresh_list fresh (snd Ys'G ∪ G) (length (fst Zs)) in
+     let ϱZ := ϱ [ fst Zs <-- Y ] in
+     let (G', s1') := renameApart' ϱZ (G ∪ snd Ys'G ∪ of_list Y) (snd Zs) in
+     ((Y, s1')::fst Ys'G, G' ∪ of_list Y ∪ snd Ys'G)).
+
+Definition renameApartF (renameApart':env var -> set var -> stmt -> set var * stmt) G ϱ
+           := fold_left (renameApartFStep renameApart' G ϱ).
+
+Definition renameApartFRight (renameApart':env var -> set var -> stmt -> set var * stmt) G ϱ
+           := fold_right (fun x y => renameApartFStep renameApart' G ϱ y x).
+
+Lemma renameApartFRight_corr renameApart' G ϱ s F
+: renameApartFRight renameApart' G ϱ s (rev F) =
+  renameApartF renameApart' G ϱ F s.
+Proof.
+  unfold renameApartF, renameApartFRight.
+  erewrite <- fold_left_rev_right; eauto.
+Qed.
+
 Fixpoint renameApart' (ϱ:env var) (G:set var) (s:stmt) : set var * stmt:=
 match s with
    | stmtLet x e s0 =>
@@ -27,34 +48,47 @@ match s with
      let ϱ' := ϱ[x <- y] in
      let (G', s') := renameApart' ϱ' {y; G} s in
        ({y; G'}, stmtExtern y f (List.map (rename_exp ϱ) Y) s')
-   | stmtFun Z s1 s2 =>
-     let Y := fresh_list fresh G (length Z) in
-     let ϱZ := ϱ [ Z <-- Y ] in
-     let (G', s1') := renameApart' ϱZ (G ∪ of_list Y) s1 in
-     let (G'', s2') := renameApart' ϱ (G ∪ (G' ∪ of_list Y)) s2 in
-     (G' ∪ (G'' ∪ of_list Y), stmtFun Y s1'  s2')
+   | stmtFun F s2 =>
+     let (F', G') := renameApartF renameApart' G ϱ F (nil, ∅) in
+     let (G'', s2') := renameApart' ϱ (G ∪ G') s2 in
+     (G' ∪ G'', stmtFun F'  s2')
    end.
+
+Lemma renamedApartF_disj renameApart' G ϱ F
+: (forall ϱ G n Zs, get F n Zs -> disj G (fst (renameApart' ϱ G (snd Zs))))
+  -> forall Ys G', disj G G' -> disj G (snd (renameApartF renameApart' G ϱ F (Ys, G'))).
+Proof.
+  general induction F; simpl; eauto.
+  - unfold renameApartFStep.
+    let_pair_case_eq; simpl_pair_eqs.
+    eapply IHF; eauto using get.
+    rewrite disj_app; split; eauto.
+    rewrite disj_app; split; eauto.
+    + subst. eapply disj_1_incl; eauto using get with cset.
+    + symmetry. eapply disj_2_incl.
+      eapply fresh_list_spec; eauto using fresh_spec with cset.
+      eauto with cset.
+Qed.
 
 Lemma renameApart'_disj ϱ G s
   : disj G (fst (renameApart' ϱ G s)).
 Proof.
-  general induction s; simpl; repeat let_pair_case_eq; simpl; subst; eauto.
+  revert ϱ G. sind s; intros; destruct s; simpl; repeat let_pair_case_eq; simpl; subst; eauto.
   - rewrite disj_add; split; eauto using fresh_spec.
-    eapply disj_subset_subset_flip_impl; [| reflexivity | eapply IHs].
-    cset_tac; intuition.
+    eapply disj_subset_subset_flip_impl; [| reflexivity | eapply (IH s)]; eauto with cset.
   - rewrite disj_app; split; eauto.
-    eapply disj_subset_subset_flip_impl; [| reflexivity | eapply IHs2].
-    cset_tac; intuition.
+    eapply disj_subset_subset_flip_impl; [| reflexivity | eapply (IH s2)]; eauto with cset.
   - rewrite disj_add; split; eauto using fresh_spec.
-    eapply disj_subset_subset_flip_impl; [| reflexivity | eapply IHs].
-    cset_tac; intuition.
+    eapply disj_subset_subset_flip_impl; [| reflexivity | eapply (IH s)]; eauto with cset.
   - repeat (rewrite disj_app; split); eauto.
-    eapply disj_subset_subset_flip_impl; [| reflexivity | eapply IHs1].
-    cset_tac; intuition.
-    eapply disj_subset_subset_flip_impl; [| reflexivity | eapply IHs2].
-    cset_tac; intuition.
-    symmetry. eapply fresh_list_spec, fresh_spec.
+    + cut (forall Ys G', disj G G' -> disj G (snd (renameApartF renameApart' G ϱ s (Ys, G')))); eauto using renamedApartF_disj.
+    + eapply disj_subset_subset_flip_impl; [| reflexivity | eapply (IH s0)]; eauto with cset.
 Qed.
+
+Definition renamedApartAnnF (renameApartAnn:stmt -> set var -> ann (set var * set var)) G
+           := fold_right (fun (Zs:params*stmt) anFG =>
+                        let ans := renameApartAnn (snd Zs) (G ∪ snd anFG ∪ of_list (fst Zs)) in
+                        (ans::fst anFG, snd (getAnn ans) ∪ of_list (fst Zs) ∪ snd anFG)).
 
 Fixpoint renamedApartAnn (s:stmt) (G:set var) : ann (set var * set var) :=
   match s with
@@ -72,117 +106,299 @@ Fixpoint renamedApartAnn (s:stmt) (G:set var) : ann (set var * set var) :=
     | stmtExtern x f Y s =>
       let an := renamedApartAnn s {x; G} in
       ann1 (G, {x; snd (getAnn an)}) an
-    | stmtFun Z s t =>
-      let ans := renamedApartAnn s (G ∪ of_list Z) in
+    | stmtFun F t =>
+      let (ans, G') := renamedApartAnnF renamedApartAnn G (nil, {}) F in
       let ant := renamedApartAnn t G in
-      ann2 (G, snd (getAnn ans) ∪ (snd (getAnn ant) ∪ of_list Z)) ans ant
+      annF (G, G' ∪ (snd (getAnn ant))) ans ant
   end.
 
+Lemma list_union_indexwise_ext X `{OrderedType X} Y (f:Y->set X) Z (g:Z -> set X) L L'
+: length L = length L'
+  -> (forall n y z, get L n y -> get L' n z -> f y [=] g z)
+  -> list_union (List.map f L) [=] list_union (List.map g L').
+Proof.
+  intros. length_equify.
+  general induction H0; simpl; eauto.
+  unfold list_union; simpl.
+  repeat rewrite list_union_start_swap.
+  rewrite IHlength_eq, H1; eauto using get; reflexivity.
+Qed.
+
+Lemma union_eq_decomp X `{OrderedType X} s s' t t'
+: s [=] s' -> t [=] t' -> s ++ t [=] s' ++ t'.
+Proof.
+  cset_tac; intros; firstorder.
+Qed.
+
+(*
 Instance renamedApart_ann_morph
 : Proper (eq ==> Equal ==> ann_R (@pe _ _ )) renamedApartAnn.
 Proof.
   unfold Proper, respectful; intros. subst.
-  general induction y; simpl; eauto using ann_R.
-  - econstructor. rewrite H0 at 1. rewrite IHy. reflexivity.
+  revert x0 y0 H0. sind y; destruct y; simpl; intros; eauto using ann_R.
+  - econstructor. rewrite H0 at 1. rewrite (IH y); eauto. reflexivity.
     rewrite H0; reflexivity.
-    eapply IHy. rewrite H0; reflexivity.
+    eapply IH; eauto. rewrite H0; reflexivity.
   - econstructor; eauto.
-    rewrite H0 at 1. rewrite IHy1, IHy2; eauto. reflexivity.
+    rewrite H0 at 1. rewrite (IH y1), (IH y2); eauto. reflexivity.
   - econstructor; rewrite H0; reflexivity.
   - econstructor; rewrite H0; reflexivity.
-  - econstructor. rewrite H0 at 1. rewrite IHy. reflexivity.
+  - econstructor. rewrite H0 at 1. rewrite (IH y); eauto. reflexivity.
     rewrite H0; reflexivity.
-    eapply IHy. rewrite H0; reflexivity.
-  - econstructor; eauto.
-    rewrite H0 at 1.
-    rewrite IHy1, IHy2; eauto. reflexivity.
-    rewrite H0; reflexivity.
-    eapply IHy1. rewrite H0; eauto.
+    eapply IH; eauto. rewrite H0; reflexivity.
+  - repeat (let_pair_case_eq; simpl_pair_eqs); subst.
+    econstructor; eauto with len.
+    + rewrite H0 at 1.
+      econstructor; eauto. rewrite IH; eauto.
+      eapply union_eq_decomp; eauto.
+      admit.
+    + admit.
+    + intros.
+      inv_map H. inv_map H1.
+    pose proof (IH (snd x)).
+    eapply ann_R_get in H5.
+    unfold comp.
+    erewrite H5. reflexivity. eauto. rewrite H0; eauto.
+    pose proof (IH y).
+    eapply ann_R_get in H; eauto.
+    rewrite H; eauto.
+    intros. inv_map H. inv_map H1.
+    eapply IH; eauto. rewrite H0; eauto.
 Qed.
+ *)
 
 Lemma fst_renamedApartAnn s G
  : fst (getAnn (renamedApartAnn s G)) = G.
 Proof.
-  general induction s; eauto.
+  sind s; destruct s; eauto.
+  - simpl. let_pair_case_eq. simpl; eauto.
 Qed.
 
-Lemma snd_renameApartAnn s G ϱ G'
+
+
+Lemma snd_renamedApartAnnF_fst G G' G'' s ϱ L L' G'''
+: (forall n Zs G ϱ G',
+     get s n Zs ->
+     snd (getAnn (renamedApartAnn (snd (renameApart' ϱ G (snd Zs))) G')) = fst (renameApart' ϱ G (snd Zs)))
+  -> snd (renamedApartAnnF renamedApartAnn G' (L', G''') L) = G''
+  ->
+   snd
+     (renamedApartAnnF renamedApartAnn
+        G' (L', G''') (fst (renameApartFRight renameApart' G ϱ (L, G'') s))) =
+   snd (renameApartFRight renameApart' G ϱ (L, G'') s).
+Proof.
+  intros.
+  revert_except s. induction s; intros.
+  - simpl. eauto.
+  - simpl.
+    unfold renameApartFStep.
+    repeat (let_pair_case_eq). simpl in *.
+    erewrite <- IHs; intros; eauto using get; try congruence.
+    subst.
+    erewrite H; eauto using get.
+Qed.
+
+Lemma get_rev X (L:list X) n x
+: get (rev L) n x ->
+  get L (length L - S n) x.
+Proof.
+  intros.
+  general induction L; simpl in *; isabsurd.
+  edestruct get_app_cases; eauto; dcr.
+  - exploit @get_length; eauto.
+    rewrite rev_length in X0; simpl in *.
+    orewrite (length L - n = S (length L - S n)).
+    eauto using get.
+  - rewrite rev_length in H2. orewrite (length L - n = 0).
+    inv H1; isabsurd; eauto using get.
+Qed.
+
+Lemma snd_renameApartAnn_fst s G ϱ G'
 : snd (getAnn (renamedApartAnn (snd (renameApart' ϱ G s)) G')) = fst (renameApart' ϱ G s).
 Proof.
-  general induction s; simpl; repeat let_pair_case_eq; simpl; eauto.
-  - subst. rewrite IHs. reflexivity.
-  - subst. rewrite IHs1. rewrite IHs2. reflexivity.
-  - subst. rewrite IHs. reflexivity.
-  - subst. rewrite IHs1. rewrite IHs2. reflexivity.
+  revert G ϱ G'.
+  sind s; destruct s; simpl; intros; repeat let_pair_case_eq; simpl; eauto.
+  - subst. rewrite (IH s); eauto.
+  - subst. rewrite (IH s1); eauto. rewrite (IH s2); eauto.
+  - subst. rewrite (IH s); eauto.
+  - subst. rewrite (IH s0); eauto.
+    let_pair_case_eq; simpl_pair_eqs; subst; simpl.
+    f_equal.
+    rewrite <- renameApartFRight_corr.
+    erewrite snd_renamedApartAnnF_fst; eauto.
+    intros. eapply get_rev in H. eauto.
+Qed.
+
+Lemma snd_renamedApartAnnF' G s
+: (forall n Zs, get s n Zs -> forall G, snd (getAnn (renamedApartAnn (snd Zs) G)) [=] definedVars (snd Zs))
+  -> snd (renamedApartAnnF renamedApartAnn G (nil, {}) s)[=]
+        list_union
+        (List.map
+           (fun f : params * stmt =>
+              (definedVars (snd f) ++ of_list (fst f))%set) s).
+Proof.
+  general induction s; simpl; eauto.
+  - rewrite H; eauto using get. unfold list_union. simpl.
+    rewrite list_union_start_swap. rewrite IHs; intros; eauto using get.
+    cset_tac; intuition.
 Qed.
 
 Lemma snd_renamedApartAnn s G
  : snd (getAnn (renamedApartAnn s G)) [=] definedVars s.
 Proof.
-  general induction s; simpl; eauto.
-  - rewrite IHs; eauto.
-  - rewrite IHs1, IHs2; eauto.
-  - rewrite IHs; eauto.
-  - rewrite IHs1, IHs2. cset_tac; intuition.
+  sinduction s; simpl; repeat rewrite H; eauto.
+  - let_pair_case_eq; simpl_pair_eqs; subst; simpl. rewrite H; eauto.
+    eapply union_eq_decomp; eauto.
+    rewrite snd_renamedApartAnnF'; eauto.
 Qed.
 
+Lemma snd_renamedApartAnnF G s
+: snd (renamedApartAnnF renamedApartAnn G (nil, {}) s)[=]
+      list_union
+      (List.map
+         (fun f : params * stmt =>
+            (definedVars (snd f) ++ of_list (fst f))%set) s).
+Proof.
+  eapply snd_renamedApartAnnF'; eauto using snd_renamedApartAnn.
+Qed.
 
 Lemma renameApartAnn_decomp s G
 : pe (getAnn (renamedApartAnn s G)) (G, snd (getAnn (renamedApartAnn s G))).
 Proof.
   destruct s; simpl; try reflexivity.
+  - let_pair_case_eq; simpl_pair_eqs; subst; simpl; eauto.
 Qed.
 
 Hint Resolve prod_eq_intro : cset.
 
-Lemma ann_R_pe_notOccur G G' s
-:  disj (occurVars s) G'
-   -> G \ G' [=] G
-   -> ann_R (@pe var _)
-           (renamedApartAnn s G)
-                     (mapAnn (pminus G') (renamedApartAnn s (G ∪ G'))).
+Lemma disj_not_in X `{OrderedType X} x s
+: disj {x} s
+  -> x ∉ s.
 Proof.
-  intros. general induction s; simpl in * |- *; try now (econstructor; reflexivity).
+  unfold disj; cset_tac.
+  intro.
+  eapply H0; eauto; intuition.
+Qed.
+
+Hint Resolve disj_not_in incl_singleton: cset.
+
+Lemma length_fst_renamedApartAnnF G F
+: length (fst (renamedApartAnnF renamedApartAnn G (nil, {}) F))
+  = length F.
+Proof.
+  general induction F; simpl; eauto.
+Qed.
+
+Lemma get_fst_renamedApartAnnF G F n ans
+:  get (fst (renamedApartAnnF renamedApartAnn G (nil, {}) F)) n ans
+   -> exists Zs G', get F n Zs
+              /\ ans = renamedApartAnn (snd Zs) G'
+              /\ G' [=] G
+                   ∪ list_union (List.map (fun f => (definedVars (snd f) ∪ of_list (fst f)))
+                                          (drop (S n) F))
+                   ∪ of_list (fst Zs).
+Proof.
+  general induction F; simpl in * |- *; isabsurd. inv H.
+  - do 2 eexists; split; eauto using get.
+    split; eauto.
+    rewrite snd_renamedApartAnnF. simpl.
+    clear_all; cset_tac; intuition.
+  - edestruct IHF as [? [? [? [? ?]]]]; eauto.
+    do 2 eexists; split; eauto using get.
+Qed.
+
+Lemma disj_eq_minus X `{OrderedType X} (s t u: set X)
+: s [=] t
+  -> disj t u
+  -> s [=] t \ u.
+Proof.
+  unfold disj.
+  cset_tac; intuition; eauto.
+  - eapply H0; eauto.
+  - eapply H1; intuition; eauto. eapply H0; eauto.
+  - eapply H0; eauto.
+Qed.
+
+Lemma union_incl_split X `{OrderedType X} s t u
+: s ⊆ u -> t ⊆ u -> s ∪ t ⊆ u.
+Proof.
+  cset_tac; intuition.
+Qed.
+
+Lemma list_union_drop_incl X `{OrderedType X} (L L':list (set X)) n
+: list_union (drop n L) ⊆ list_union (drop n L')
+  -> list_union (drop n L) ⊆ list_union L'.
+Proof.
+  intros; hnf; intros.
+  eapply H0 in H1.
+  edestruct list_union_get; eauto; dcr.
+  eapply incl_list_union; eauto using get_drop; reflexivity.
+  cset_tac; intuition.
+Qed.
+
+Lemma ann_R_pe_notOccur G1 G2 G' s
+:  disj (occurVars s) G'
+   -> G1 [=] G2 \ G'
+   -> ann_R (@pe var _)
+           (renamedApartAnn s G1)
+           (mapAnn (pminus G') (renamedApartAnn s G2)).
+Proof.
+  revert G1 G2 G'.
+  sind s; destruct s; intros; simpl in * |- *; eauto using pe, ann_R with cset;
+  try now (econstructor; reflexivity).
   - econstructor.
-    + econstructor; eauto. rewrite minus_dist_union. rewrite H0.
-      cset_tac; intuition. repeat rewrite snd_renamedApartAnn; eauto.
-    + assert ({x ; G ++ G'} [=] {x; G} ++ G'). {
-        cset_tac; intuition.
-      } rewrite H1. eapply IHs; eauto with cset.
-      admit.
+    + econstructor; eauto.
+      repeat rewrite snd_renamedApartAnn; eauto.
+    + eapply IH; eauto with cset.
+      rewrite H0.
+      assert (x ∉ G'). eauto with cset.
+      revert H1; clear_all; cset_tac; intuition.
   - econstructor; eauto with cset.
-    + rewrite IHs1, IHs2; eauto with cset;
-      repeat rewrite getAnn_mapAnn.
-      unfold pminus.
-      repeat let_pair_case_eq; simpl; subst; eauto.
-      econstructor; try reflexivity.
-      rewrite minus_dist_union. rewrite H0. cset_tac; intuition.
+    + repeat rewrite snd_renamedApartAnn; eauto.
+      econstructor; eauto.
   - econstructor; eauto with cset. econstructor; eauto.
-    rewrite minus_dist_union. rewrite H0. cset_tac; intuition.
   - econstructor. econstructor; try rewrite <- H0; clear_all; cset_tac; intuition.
-  - assert ({x ; G ++ G'} [=] {x; G} ++ G'). {
-      cset_tac; intuition.
-    }
-    econstructor; eauto with cset.
+  - econstructor; eauto with cset.
     + econstructor; eauto.
-      * rewrite minus_dist_union. rewrite H0.
-        cset_tac; intuition.
-      * repeat rewrite snd_renamedApartAnn; eauto.
-    + assert ({x ; G ++ G'} [=] {x; G} ++ G'). {
-        cset_tac; intuition.
-      } rewrite H1. eapply IHs; eauto with cset.
-      admit.
-  - assert ((G ++ G') ++ of_list Z [=] (G ++ of_list Z) ++ G'). {
-      cset_tac; intuition.
-    }
+      repeat rewrite snd_renamedApartAnn; eauto.
+    + eapply IH; eauto with cset.
+      assert (x ∉ G'). eauto with cset.
+      rewrite H0. revert H1; clear_all; cset_tac; intuition.
+  - intros.
+    repeat let_pair_case_eq; subst; simpl.
     econstructor; eauto with cset.
-    + econstructor; eauto.
-      * rewrite minus_dist_union. rewrite H0. cset_tac; intuition.
-      * repeat rewrite snd_renamedApartAnn; eauto.
-    + rewrite H1. eapply IHs1; eauto with cset.
-      rewrite minus_dist_union, H0.
-      rewrite minus_inane_set; eauto.
-      eapply disj_1_incl; eauto with cset.
+    + repeat rewrite snd_renamedApartAnn.
+      unfold pminus. econstructor; eauto.
+      eapply union_eq_decomp; eauto.
+      repeat rewrite snd_renamedApartAnnF; eauto.
+    + rewrite List.map_length; eauto.
+      repeat rewrite length_fst_renamedApartAnnF; eauto.
+    + intros.
+      inv_map H2.
+      edestruct get_fst_renamedApartAnnF as [? [? ?]]; dcr; eauto. subst.
+      edestruct get_fst_renamedApartAnnF as [? [? ?]]; dcr; try eapply H1; eauto. subst.
+      get_functional; subst.
+      eapply IH; eauto.
+      * eapply disj_1_incl; eauto. unfold list_union.
+        eapply incl_union_left.
+        eapply incl_list_union; eauto using map_get_1 with cset.
+      * rewrite H11, H9.
+        repeat rewrite minus_dist_union.
+        setoid_rewrite union_assoc at 2.
+        setoid_rewrite <- minus_dist_union.
+        rewrite union_assoc.
+        eapply union_eq_decomp; eauto.
+        eapply disj_eq_minus; eauto.
+        eapply disj_1_incl; eauto.
+        eapply incl_union_left.
+        eapply union_incl_split.
+        rewrite drop_map.
+        eapply list_union_drop_incl.
+        repeat rewrite <- drop_map.
+        eapply list_union_f_incl; intros.
+        rewrite occurVars_freeVars_definedVars. cset_tac; intuition.
+        eapply incl_list_union. eapply map_get_1; eauto.
+        cset_tac; intuition.
 Qed.
 
 
@@ -195,13 +411,40 @@ Proof.
   clear_all. general induction Y; simpl; eauto using AllInRel.PIR2, freeVars_renameExp.
 Qed.
 
+Lemma definedVars_renamedApart' ϱ G s
+: definedVars (snd (renameApart' ϱ G s)) [=] fst (renameApart' ϱ G s).
+Proof.
+  revert ϱ G.
+  sind s; destruct s; intros; simpl; repeat let_pair_case_eq; simpl in * |- *; subst; eauto;
+  repeat rewrite lookup_set_union; try rewrite freeVars_renameExp; eauto;
+  repeat rewrite IH; eauto; try reflexivity.
+  eapply union_eq_decomp; eauto.
+  rewrite <- renameApartFRight_corr.
+  remember (rev s).
+  assert (forall n Zs, get l n Zs -> exists n', get s n' Zs).
+  intros. subst. eapply get_rev in H. eauto. clear Heql.
+  general induction l.
+  - reflexivity.
+  - simpl.
+    unfold renameApartFStep. let_pair_case_eq.
+    simpl_pair_eqs. subst. simpl.
+    unfold list_union. simpl. rewrite list_union_start_swap.
+    simpl.
+    eapply union_eq_decomp; eauto.
+    + edestruct H; eauto using get.
+      rewrite IH; eauto. cset_tac; intuition.
+    + eapply IHl; eauto using get.
+Qed.
+
+
 Lemma freeVars_renamedApart' ϱ G s
 : lookup_set ϱ (freeVars s) ⊆ G
   -> freeVars (snd (renameApart' ϱ G s)) [=] lookup_set ϱ (freeVars s).
 Proof.
-  general induction s; simpl; repeat let_pair_case_eq; simpl in * |- *; subst; eauto;
+  revert G ϱ.
+  sind s; destruct s; intros; simpl; repeat let_pair_case_eq; simpl in * |- *; subst; eauto;
           repeat rewrite lookup_set_union; try rewrite freeVars_renameExp; eauto; try reflexivity.
-  - rewrite IHs.
+  - rewrite IH; eauto.
     + rewrite lookup_set_update_union_minus; eauto.
       assert (fresh G ∉ lookup_set ϱ (freeVars s \ {{x}})).
       intro. eapply lookup_set_incl in H0; eauto.
@@ -211,12 +454,11 @@ Proof.
     + rewrite lookup_set_update_in_union; eauto.
       rewrite <- H at 3. repeat rewrite lookup_set_union; eauto.
       cset_tac; intuition.
-  - rewrite IHs1, IHs2.
-    + reflexivity.
+  - repeat rewrite IH; eauto.
     + rewrite <- H at 1. repeat rewrite lookup_set_union; eauto. cset_tac; intuition.
     + rewrite <- H at 1. repeat rewrite lookup_set_union; eauto. cset_tac; intuition.
   - eapply freeVars_rename_exp_list.
-  - rewrite IHs.
+  - rewrite IH; eauto.
     + rewrite freeVars_rename_exp_list.
       rewrite lookup_set_update_union_minus; eauto.
       assert (fresh G ∉ lookup_set ϱ (freeVars s \ {{x}})).
@@ -227,7 +469,37 @@ Proof.
     + rewrite lookup_set_update_in_union; eauto.
       rewrite <- H at 3. repeat rewrite lookup_set_union; eauto.
       cset_tac; intuition.
-  - rewrite IHs1, IHs2.
+  - eapply union_eq_decomp; eauto.
+    + unfold list_union.
+      rewrite lookup_set_list_union; eauto; try reflexivity.
+      rewrite map_map.
+      Lemma list_union_rev X `{OrderedType X} (L:list (set X)) s
+      : fold_left union L s [=] fold_left union (rev L) s.
+      Proof.
+        general induction L; simpl; eauto.
+        rewrite list_union_app.
+        unfold list_union. simpl.
+        rewrite IHL.
+        repeat rewrite list_union_start_swap.
+        cset_tac; intuition.
+      Qed.
+      intros. setoid_rewrite list_union_rev at 2.
+      rewrite <- map_rev.
+      eapply list_union_indexwise_ext.
+      Lemma renameApartF_length G ϱ F
+      : length (fst (renameApartF renameApart' G ϱ F (nil, {}))) = length F.
+      Proof.
+        rewrite <- renameApartFRight_corr.
+        rewrite <- (rev_length F).
+        generalize (rev F); intros; clear F.
+        general induction l; simpl; eauto.
+        unfold renameApartFStep; simpl.
+        let_pair_case_eq; simpl_pair_eqs; subst; simpl; eauto.
+      Qed.
+      rewrite renameApartF_length; eauto.
+      intros.
+      (*
+    rewrite IHs1, IHs2.
     + rewrite lookup_set_update_union_minus_list; eauto.
       rewrite lookup_set_union in H; eauto.
       pose proof (fresh_list_spec _ fresh_spec G (length Z)).
@@ -239,19 +511,122 @@ Proof.
       cset_tac; intuition.
     + rewrite lookup_set_update_with_list_in_union_length; eauto.
       rewrite <- H at 2. rewrite lookup_set_union; eauto. cset_tac; intuition.
+      rewrite fresh_list_length; eauto.*)
+      intros.
+Lemma get_fst_renameApartF G ϱ F n ans
+:  get (fst (renameApartF renameApart' G ϱ F (nil, {}))) n ans
+   -> exists ϱ' Zs G', get F (length F - S n) Zs
+                 /\ snd ans = snd (renameApart' ϱ' G' (snd Zs))
+                 /\ G ⊆ G'
+                 /\ lookup_set ϱ' (of_list (fst Zs)) ⊆ of_list (fst ans)
+                 /\ of_list (fst ans) ⊆ G'
+                 /\ agree_on eq (freeVars (snd Zs) \ of_list (fst Zs)) ϱ ϱ'
+                 /\ disj G (of_list (fst ans)).
+Proof.
+  rewrite <- renameApartFRight_corr.
+  remember (rev F).
+  general induction l; simpl in * |- *; isabsurd.
+  - unfold renameApartFStep in *.
+    revert H; let_pair_case_eq; simpl_pair_eqs.
+    inv H0; subst.
+    + do 3 eexists; split; eauto using get.
+      eapply get_rev. rewrite <- Heql. econstructor.
+      simpl. split. reflexivity.
+      split. cset_tac; intuition.
+      Lemma update_with_list_lookup_list_incl {X} `{OrderedType X} {Y} `{OrderedType Y} (f:X->Y)
+      `{Proper _ (_eq ==> _eq) f} Z Z'
+: length Z = length Z'
+  -> lookup_set (f [ Z <-- Z' ]) (of_list Z) ⊆ of_list Z'.
+      Proof.
+        intros. hnf; intros.
+        eapply lookup_set_spec in H3; eauto; dcr.
+        rewrite H6.
+        eapply update_with_list_lookup_in; eauto.
+      Qed.
+      split.
+      rewrite update_with_list_lookup_list_incl; eauto.
       rewrite fresh_list_length; eauto.
+      split. eauto.
+      split.
+      symmetry.
+      eapply update_with_list_agree_minus; eauto.
+      rewrite fresh_list_length; eauto.
+      Lemma lookup_set_update_disj {X} `{OrderedType X} {Y} `{OrderedType Y} (f:X->Y)
+            `{Proper _ (_eq ==> _eq) f} Z Z' G
+      : disj (of_list Z) G
+        -> lookup_set (f [ Z <-- Z' ]) G [=] lookup_set f G.
+      Proof.
+        intros. hnf; intros.
+        rewrite lookup_set_spec; eauto.
+        split; intuition; dcr. rewrite H6.
+        - rewrite lookup_set_update_not_in_Z; eauto.
+          eapply lookup_set_spec; eauto.
+        - eapply lookup_set_spec in H3; eauto; dcr.
+          eexists x.
+          rewrite lookup_set_update_not_in_Z; eauto.
+      Qed.
+      intros.
+      symmetry. eapply disj_2_incl.
+      eapply fresh_list_spec. eapply fresh_spec. eauto.
+    + edestruct IHl as [? [? [? [? ?]]]]; eauto.
+      instantiate (1:=rev (tl (rev F))). rewrite <- Heql. simpl. rewrite rev_involutive; eauto.
+      rewrite <- Heql in *. simpl in *.
+      assert (S (length (rev l)) = length (rev F)).
+      rewrite <- Heql. simpl. rewrite rev_length; eauto.
+      do 3 eexists; split; eauto using get.
+      assert (length F = S (length (rev l))).
+      rewrite rev_length.
+      rewrite <- rev_length. rewrite <- Heql. eauto.
+      Lemma rev_swap X (L L':list X)
+      : rev L = L'
+        -> L = rev L'.
+      Proof.
+        intros. subst. rewrite rev_involutive; eauto.
+      Qed.
+      exploit rev_swap. symmetry; eauto. simpl in *.
+      rewrite X at 1. eapply get_app.
+      rewrite H3. simpl. eauto.
+Qed.
+rewrite rev_length; eauto.
+intros.
+edestruct get_fst_renameApartF as [? [? [? ?]]]; dcr; eauto.
+eapply get_rev in H1. get_functional; subst.
+rewrite H5.
+rewrite IH; eauto.
+      * assert (freeVars (snd x0) [=] (freeVars (snd x0) \ of_list (fst x0)) ∪ (of_list (fst x0) ∩ freeVars (snd x0))).
+        clear_all; cset_tac; intuition. simpl in *.
+        decide (a ∈ of_list a0); intuition.
+        rewrite H1 at 1. repeat rewrite lookup_set_union; eauto.
+        repeat rewrite minus_dist_union.
+        rewrite <- lookup_set_agree; eauto.
+        Lemma disj_minus_eq X `{OrderedType X} (s t:set X)
+        : disj s t
+          -> s \ t [=] s.
+        Proof.
+          unfold disj; cset_tac; intuition; eauto.
+        Qed.
+        intros. rewrite disj_minus_eq.
+        setoid_rewrite diff_subset_equal at 2. cset_tac; intuition.
+        rewrite meet_incl; eauto.
+        eapply disj_1_incl; eauto.
+        rewrite <- H. eapply lookup_set_incl; eauto.
+        eapply incl_union_left. eapply incl_list_union; eauto.
+        eapply map_get_1; eauto. eauto.
+      * assert (freeVars (snd x0) ⊆ (freeVars (snd x0) \ of_list (fst x0)) ∪ of_list (fst x0)).
+        clear_all; cset_tac; intuition.
+        decide (a ∈ of_list (fst x0)); eauto.
+        rewrite H1. rewrite lookup_set_union; eauto. rewrite H6.
+        eapply union_subset_3; eauto.
+        rewrite <- H4. rewrite <- H.
+        rewrite <- lookup_set_agree; eauto.
+        eapply lookup_set_incl; eauto.
+        eapply incl_union_left.
+        eapply incl_list_union; eauto.
+        eapply map_get_1; eauto. eauto.
+    + rewrite IH; eauto. eapply incl_union_left. rewrite <- H.
+      eapply lookup_set_incl; eauto.
 Qed.
 
-Lemma definedVars_renamedApart' ϱ G s
-: definedVars (snd (renameApart' ϱ G s)) [=] fst (renameApart' ϱ G s).
-Proof.
-  general induction s; simpl; repeat let_pair_case_eq; simpl in * |- *; subst; eauto;
-          repeat rewrite lookup_set_union; try rewrite freeVars_renameExp; eauto; try reflexivity.
-  - rewrite IHs; eauto; reflexivity.
-  - rewrite IHs1, IHs2; reflexivity.
-  - rewrite IHs; reflexivity.
-  - rewrite IHs1, IHs2. rewrite union_assoc. reflexivity.
-Qed.
 
 
 Lemma renameApart'_renamedApart (s:stmt) ϱ G
